util/vfmTypesScript.sml
@@ -1,6 +1,6 @@
 Theory vfmTypes
 Ancestors
-  arithmetic byte cv_std divides list rich_list combin numposrep words
+  arithmetic byte cv_std divides list rich_list sptree combin numposrep words
   keccak
 Libs
   blastLib
@@ -19,6 +19,28 @@ Theorem prod_CASE_rator =
 Theorem sum_CASE_rator =
   DatatypeSimps.mk_case_rator_thm_tyinfo
     (Option.valOf (TypeBase.read {Thy="sum",Tyop="sum"}));
+
+(* TODO: move to sptree? like MAP FST (toAList t) but ignores values *)
+Definition domain_list_def:
+  domain_list LN = [] ∧
+  domain_list (LS _) = [0n] ∧
+  domain_list (BN t1 t2) =
+     MAP (λn. 2 * n + 2) (domain_list t1) ++
+     MAP (λn. 2 * n + 1) (domain_list t2) ∧
+  domain_list (BS t1 v t2) =
+     0::
+     MAP (λn. 2 * n + 2) (domain_list t1) ++
+     MAP (λn. 2 * n + 1) (domain_list t2)
+End
+
+val () = cv_auto_trans domain_list_def;
+
+Theorem set_domain_list:
+  set (domain_list t) = domain t
+Proof
+  Induct_on`t` \\ rw[domain_list_def, LIST_TO_SET_MAP]
+  \\ rw[pred_setTheory.EXTENSION] \\ metis_tac[]
+QED
 
 val () = cv_trans (word_of_bytes_le_eq_num_of_bytes |> INST_TYPE [alpha |-> “:160”] |> SRULE[compute_divides]);
 val () = cv_trans (word_of_bytes_be_eq_num_of_bytes |> INST_TYPE [alpha |-> “:160”] |> SRULE[compute_divides]);
